try to fix the random seed example

sum-random/SeedRefinement.thy
@@ -1,7 +1,7 @@
 theory SeedRefinement
 imports "lib/CogentMonad"
         "lib/CogentCorres"
-        "build_random_seed/Random_seed_AllRefine"
+        "build/Random_seed_AllRefine"
 begin        
 
 section\<open> The shallow Cogent code refines a non-deterministic monad representing the set of all values \<close>
@@ -12,7 +12,7 @@ text \<open>This is trivial to prove as any program refines the set of all value
 
 
 abbreviation "rand_with_seed_spec \<equiv> UNIV:: 64 word cogent_monad"
-abbreviation "main_spec \<equiv> UNIV:: 64 word cogent_monad"
+abbreviation "sum_spec \<equiv> UNIV:: 64 word cogent_monad"
 
 abbreviation "val_rel_monadic_shallow \<equiv> (\<lambda>(v:: 'b) sv:: ('a, 'b) SeedValue. v =  value\<^sub>f sv)"
 
@@ -28,8 +28,8 @@ lemma rand_with_seed_corres_monad_shallow :
 by(simp add:cogent_corres_def)
 
 (*NOTE that this is trivial -- any function would satisfy this spec *)
-lemma main_corres_monad_shallow :
-  "\<And>s. cogent_corres val_rel_monadic_shallow main_spec (Random_seed_Shallow_Desugar.main s)"
+lemma sum_corres_monad_shallow :
+  "\<And>s. cogent_corres val_rel_monadic_shallow sum_spec (Random_seed_Shallow_Desugar.sum s)"
   by(simp add:cogent_corres_def)
 
 
@@ -40,12 +40,12 @@ section\<open>Refinement proofs of abstract functions from C to shallow Cogent\<
 
 
 term "correspondence (\<lambda>a. ([],[])) (\<lambda>a b c d. False) (\<lambda>a b c d e f g h. False) (\<lambda>a b c d e f g h i. False)"
-thm Random_seed_AllRefine.Random_seed_cogent_shallow.corres_shallow_C_main[no_vars]
+thm Random_seed_AllRefine.Random_seed_cogent_shallow.corres_shallow_C_sum[no_vars]
 thm random_seed.rand_with_seed'_def
 
 thm Random_seed_cogent_shallow_def
 
-lemma corres_shallow_C_main_no_assms:
+lemma corres_shallow_C_sum_no_assms:
   "Random_seed_cogent_shallow abs_repr val_abs_typing upd_abs_typing abs_upd_val \<Longrightarrow>
 (\<And>i \<gamma> v' \<Gamma>' \<sigma> st.
     i < length \<gamma> \<Longrightarrow>
@@ -56,7 +56,7 @@ lemma corres_shallow_C_main_no_assms:
                     (do x <- random_seed.rand_with_seed' v';
                               gets (\<lambda>s. x)
                      od)
-     \<xi>_0 \<gamma> (assoc_lookup [(''rand_with_seed'', Random_seed_TypeProof.rand_with_seed_type), (''main'', Random_seed_TypeProof.main_type)] (0, [], {}, TUnit, TUnit)) \<Gamma>' \<sigma>
+     \<xi>_0 \<gamma> (assoc_lookup [(''rand_with_seed'', Random_seed_TypeProof.rand_with_seed_type), (''sum'', Random_seed_TypeProof.sum_type)] (0, [], {}, TUnit, TUnit)) \<Gamma>' \<sigma>
      st) \<Longrightarrow>
 correspondence_init abs_repr val_abs_typing upd_abs_typing abs_upd_val \<Longrightarrow>
 value_sem.rename_mono_prog val_abs_typing rename \<Xi> \<xi>\<^sub>m \<xi>\<^sub>p \<Longrightarrow>
@@ -64,9 +64,9 @@ vv\<^sub>m = value_sem.rename_val rename (value_sem.monoval vv\<^sub>p) \<Longri
 correspondence_init.val_rel_shallow_C abs_repr abs_upd_val rename vv\<^sub>s uv\<^sub>C vv\<^sub>p uv\<^sub>m \<xi>\<^sub>p \<sigma> \<Xi> \<Longrightarrow>
 proc_ctx_wellformed \<Xi> \<Longrightarrow>
 value_sem.proc_env_matches val_abs_typing \<xi>\<^sub>m \<Xi> \<Longrightarrow>
-value_sem.matches val_abs_typing \<Xi> [vv\<^sub>m] [Some (fst (snd (snd (snd Random_seed_TypeProof.main_type))))] \<Longrightarrow>
-correspondence_init.corres_shallow_C abs_repr upd_abs_typing abs_upd_val rename Random_seed.state_rel (Random_seed_Shallow_Desugar.main vv\<^sub>s) Random_seed_TypeProof.main
- (random_seed.main' uv\<^sub>C) \<xi>_0 \<xi>\<^sub>m \<xi>\<^sub>p [uv\<^sub>m] [vv\<^sub>m] \<Xi> [Some (fst (snd (snd (snd Random_seed_TypeProof.main_type))))] \<sigma> s
+value_sem.matches val_abs_typing \<Xi> [vv\<^sub>m] [Some (fst (snd (snd (snd Random_seed_TypeProof.sum_type))))] \<Longrightarrow>
+correspondence_init.corres_shallow_C abs_repr upd_abs_typing abs_upd_val rename Random_seed.state_rel (Random_seed_Shallow_Desugar.sum vv\<^sub>s) Random_seed_TypeProof.sum
+ (random_seed.sum' uv\<^sub>C) \<xi>_0 \<xi>\<^sub>m \<xi>\<^sub>p [uv\<^sub>m] [vv\<^sub>m] \<Xi> [Some (fst (snd (snd (snd Random_seed_TypeProof.sum_type))))] \<sigma> s
   [cogent_C_heap]"
-theorem main_corres_monad_C:
+
 
